src/Reflection/Z/Syntax.v
@@ -6,13 +6,11 @@ Export Syntax.Notations.
 
 Local Set Boolean Equality Schemes.
 Local Set Decidable Equality Schemes.
-Inductive base_type := TZ.
-
-Local Notation tZ := (Tbase TZ).
+Inductive base_type := TZ | TWord (logsz : nat).
 
 Definition interp_base_type (v : base_type) : Type :=
   match v with
-  | TZ => Z
+  | _ => Z
   end.
 
 Inductive op : flat_type base_type -> flat_type base_type -> Type :=
@@ -31,11 +29,11 @@ Inductive op : flat_type base_type -> flat_type base_type -> Type :=
 
 Definition interpToZ {t} : interp_base_type t -> Z
   := match t with
-     | TZ => fun x => x
+     | _ => fun x => x
      end.
 Definition ZToInterp {t} : Z -> interp_base_type t
   := match t return Z -> interp_base_type t with
-     | TZ => fun x => x
+     | _ => fun x => x
      end.
 Definition cast_const {t1 t2} (v : interp_base_type t1) : interp_base_type t2
   := ZToInterp (interpToZ v).
@@ -47,15 +45,15 @@ Local Notation eta4 x := (eta3 (fst x), snd x).
 Definition interp_op src dst (f : op src dst) : interp_flat_type interp_base_type src -> interp_flat_type interp_base_type dst
   := match f in op src dst return interp_flat_type interp_base_type src -> interp_flat_type interp_base_type dst with
      | OpConst _ v => fun _ => v
-     | Add TZ => fun xy => fst xy + snd xy
-     | Sub TZ => fun xy => fst xy - snd xy
-     | Mul TZ => fun xy => fst xy * snd xy
-     | Shl TZ => fun xy => Z.shiftl (fst xy) (snd xy)
-     | Shr TZ => fun xy => Z.shiftr (fst xy) (snd xy)
-     | Land TZ => fun xy => Z.land (fst xy) (snd xy)
-     | Lor TZ => fun xy => Z.lor (fst xy) (snd xy)
-     | Neg TZ int_width => fun x => ModularBaseSystemListZOperations.neg int_width x
-     | Cmovne TZ => fun xyzw => let '(x, y, z, w) := eta4 xyzw in cmovne x y z w
-     | Cmovle TZ => fun xyzw => let '(x, y, z, w) := eta4 xyzw in cmovl x y z w
+     | Add _ => fun xy => fst xy + snd xy
+     | Sub _ => fun xy => fst xy - snd xy
+     | Mul _ => fun xy => fst xy * snd xy
+     | Shl _ => fun xy => Z.shiftl (fst xy) (snd xy)
+     | Shr _ => fun xy => Z.shiftr (fst xy) (snd xy)
+     | Land _ => fun xy => Z.land (fst xy) (snd xy)
+     | Lor _ => fun xy => Z.lor (fst xy) (snd xy)
+     | Neg _ int_width => fun x => ModularBaseSystemListZOperations.neg int_width x
+     | Cmovne _ => fun xyzw => let '(x, y, z, w) := eta4 xyzw in cmovne x y z w
+     | Cmovle _ => fun xyzw => let '(x, y, z, w) := eta4 xyzw in cmovl x y z w
      | Cast _ _ => cast_const
      end%Z.
