src/Reflection/Z/JavaNotations.v
@@ -14,7 +14,6 @@ Reserved Notation "'M32' & x" (at level 200, x at level 9).
 Global Open Scope expr_scope.
 
 Notation "T x = A ; b" := (LetIn (tx:=T) A (fun x => b)) : expr_scope.
-(*
 Notation "'int'" := (Tbase (TWord 0)).
 Notation "'int'" := (Tbase (TWord 1)).
 Notation "'int'" := (Tbase (TWord 2)).
@@ -39,7 +38,6 @@ Notation "'(int)' x" := (Op (Cast _ (TWord 4)) (Var x)).
 Notation "'(int)' x" := (Op (Cast _ (TWord 5)) (Var x)).
 Notation "'M32' & x" := (Op (Cast _ (TWord 6)) (Var x)).
 Notation "'(uint128_t)' x" := (Op (Cast _ (TWord 7)) (Var x)).
-*)
 Notation "x + y" := (Op (Add _) (Pair x y)).
 Notation "x + y" := (Op (Add _) (Pair (Var x) y)).
 Notation "x + y" := (Op (Add _) (Pair x (Var y))).
@@ -65,7 +63,6 @@ for opn, op in (('*', 'Mul'), ('+', 'Add'), ('&', 'Land')):
                     rhs = (rhs if side != 'r' else '(Op (Cast _ (TWord %d)) %s)' % (lgwordsz, rhs))
                     print('Notation "x %s y" := (Op (%s (TWord %d)) (Pair %s %s)).' % (opn, op, lgwordsz, lhs, rhs))
 >> *)
-(*
 Notation "x * y" := (Op (Mul (TWord 5)) (Pair (Op (Cast _ (TWord 5)) x) y)).
 Notation "x * y" := (Op (Mul (TWord 5)) (Pair (Op (Cast _ (TWord 5)) x) (Var y))).
 Notation "x * y" := (Op (Mul (TWord 5)) (Pair (Op (Cast _ (TWord 5)) (Var x)) y)).
@@ -114,7 +111,6 @@ Notation "x + y" := (Op (Add (TWord 7)) (Pair x (Op (Cast _ (TWord 7)) y))).
 Notation "x + y" := (Op (Add (TWord 7)) (Pair x (Op (Cast _ (TWord 7)) (Var y)))).
 Notation "x + y" := (Op (Add (TWord 7)) (Pair (Var x) (Op (Cast _ (TWord 7)) y))).
 Notation "x + y" := (Op (Add (TWord 7)) (Pair (Var x) (Op (Cast _ (TWord 7)) (Var y)))).
-*)
 Notation "x >>> y" := (Op (Shr _) (Pair x y)).
 Notation "x >>> y" := (Op (Shr _) (Pair (Var x) y)).
 Notation "x >>> y" := (Op (Shr _) (Pair x (Var y))).
@@ -127,7 +123,6 @@ Notation "x & y" := (Op (Land _) (Pair x y)).
 Notation "x & y" := (Op (Land _) (Pair (Var x) y)).
 Notation "x & y" := (Op (Land _) (Pair x (Var y))).
 Notation "x & y" := (Op (Land _) (Pair (Var x) (Var y))).
-(*
 Notation "x & y" := (Op (Land (TWord 6)) (Pair (Op (Cast _ (TWord 6)) x) y)).
 Notation "x & y" := (Op (Land (TWord 6)) (Pair (Op (Cast _ (TWord 6)) x) (Var y))).
 Notation "x & y" := (Op (Land (TWord 6)) (Pair (Op (Cast _ (TWord 6)) (Var x)) y)).
@@ -144,6 +139,5 @@ Notation "x & y" := (Op (Land (TWord 7)) (Pair x (Op (Cast _ (TWord 7)) y))).
 Notation "x & y" := (Op (Land (TWord 7)) (Pair x (Op (Cast _ (TWord 7)) (Var y)))).
 Notation "x & y" := (Op (Land (TWord 7)) (Pair (Var x) (Op (Cast _ (TWord 7)) y))).
 Notation "x & y" := (Op (Land (TWord 7)) (Pair (Var x) (Op (Cast _ (TWord 7)) (Var y)))).
-*)
 Notation Return x := (Var x).
 Notation Java_like := (Expr base_type op _).
